isabelle/type_system/BabKindcheck.thy
@@ -1,5 +1,5 @@
 theory BabKindcheck
-  imports "TypeEnv" "../base/IntRange"
+  imports "TypeEnv" "../base/IntRange" TypeProps
 begin
 
 (* This file defines well-kindedness for types. We only have one kind, *, because
@@ -47,14 +47,15 @@ definition dims_in_range :: "BabDimension list \<Rightarrow> bool" where
 definition array_dims_well_kinded :: "BabDimension list \<Rightarrow> bool" where
   "array_dims_well_kinded dims \<equiv> dims_uniform dims \<and> dims_in_range dims"
 
+(* Definition: ty is well-kinded in env. *)
 fun is_well_kinded :: "BabTyEnv \<Rightarrow> BabType \<Rightarrow> bool" where
   "is_well_kinded env (BabTy_Name loc typeName argTypes) =
     (if typeName |\<in>| TE_TypeVars env then
        argTypes = []
      else
        (case fmlookup (TE_Datatypes env) typeName of
-         Some dt \<Rightarrow> length argTypes = length (DD_TyArgs dt)
-                    \<and> list_all (is_well_kinded env) argTypes
+         Some tyVars \<Rightarrow> length argTypes = length tyVars
+                        \<and> list_all (is_well_kinded env) argTypes
        | None \<Rightarrow> False))"
 
 | "is_well_kinded env (BabTy_Bool loc) = True"
@@ -78,5 +79,302 @@ using assms by (cases ty) auto
 lemma list_all_is_well_kinded_meta:
   "list_all (is_well_kinded env) (map BabTy_Meta xs)"
   by (induction xs) simp_all
+
+
+(* Adding type variables to the environment preserves well-kindedness,
+   provided the new type variables don't shadow datatype names *)
+lemma is_well_kinded_extend_tyvars:
+  assumes "is_well_kinded env ty"
+      and "extra |\<inter>| fmdom (TE_Datatypes env) = {||}"
+  shows "is_well_kinded (env \<lparr> TE_TypeVars := TE_TypeVars env |\<union>| extra \<rparr>) ty"
+using assms proof (induction ty rule: measure_induct_rule[where f=bab_type_size])
+  case (less ty)
+  let ?extEnv = "env \<lparr> TE_TypeVars := TE_TypeVars env |\<union>| extra \<rparr>"
+  show ?case
+  proof (cases ty)
+    case (BabTy_Name loc name argTypes)
+    from less.prems(1) BabTy_Name show ?thesis
+    proof (cases "name |\<in>| TE_TypeVars env")
+      case True
+      (* name is a type variable in env, so also in extended env *)
+      with less.prems(1) BabTy_Name have "argTypes = []" by simp
+      moreover have "name |\<in>| TE_TypeVars ?extEnv"
+        using True by simp
+      ultimately show ?thesis using BabTy_Name by simp
+    next
+      case False
+      (* name is not a type variable in env, so must be a datatype in env *)
+      with less.prems(1) BabTy_Name obtain dtTyVars where
+        dt_lookup: "fmlookup (TE_Datatypes env) name = Some dtTyVars" and
+        len_eq: "length argTypes = length dtTyVars" and
+        args_wk: "list_all (is_well_kinded env) argTypes"
+        by (auto split: option.splits)
+      (* name is a datatype, so it's not in extra (by the non-shadowing assumption) *)
+      from dt_lookup have "name |\<in>| fmdom (TE_Datatypes env)"
+        by (simp add: fmdomI)
+      with less.prems(2) have "name |\<notin>| extra"
+        by auto
+      with False have not_tyvar_ext: "name |\<notin>| TE_TypeVars ?extEnv"
+        by simp
+      (* By IH, args are well-kinded in extended env *)
+      have args_wk_ext: "list_all (is_well_kinded ?extEnv) argTypes"
+      proof (simp add: list_all_iff, intro ballI)
+        fix t assume t_in: "t \<in> set argTypes"
+        from t_in BabTy_Name have "bab_type_size t < bab_type_size ty"
+          using bab_type_smaller_than_list by simp
+        moreover from args_wk t_in have "is_well_kinded env t"
+          by (simp add: list_all_iff)
+        ultimately show "is_well_kinded ?extEnv t"
+          using less.IH less.prems(2) by blast
+      qed
+      (* TE_Datatypes is unchanged between env and extEnv *)
+      have dt_lookup_ext: "fmlookup (TE_Datatypes ?extEnv) name = Some dtTyVars"
+        using dt_lookup by simp
+      with not_tyvar_ext len_eq args_wk_ext BabTy_Name show ?thesis by simp
+    qed
+  next
+    case (BabTy_Tuple loc tys)
+    from less.prems(1) BabTy_Tuple have tys_wk: "list_all (is_well_kinded env) tys"
+      by simp
+    have "list_all (is_well_kinded ?extEnv) tys"
+    proof (simp add: list_all_iff, intro ballI)
+      fix t assume t_in: "t \<in> set tys"
+      from t_in BabTy_Tuple have "bab_type_size t < bab_type_size ty"
+        using bab_type_smaller_than_list by simp
+      moreover from tys_wk t_in have "is_well_kinded env t"
+        by (simp add: list_all_iff)
+      ultimately show "is_well_kinded ?extEnv t"
+        using less.IH less.prems(2) by blast
+    qed
+    with BabTy_Tuple show ?thesis by simp
+  next
+    case (BabTy_Record loc flds)
+    from less.prems(1) BabTy_Record have flds_wk: "list_all (is_well_kinded env \<circ> snd) flds"
+      by simp
+    have "list_all (is_well_kinded ?extEnv \<circ> snd) flds"
+    proof (simp add: list_all_iff, intro ballI)
+      fix fld assume fld_in: "fld \<in> set flds"
+      from fld_in BabTy_Record have "bab_type_size (snd fld) < bab_type_size ty"
+        using bab_type_smaller_than_fieldlist
+        by (metis bab_type_size.simps(7) plus_1_eq_Suc prod.exhaust_sel)
+      moreover from flds_wk fld_in have "is_well_kinded env (snd fld)"
+        by (simp add: list_all_iff)
+      ultimately show "is_well_kinded ?extEnv (snd fld)"
+        using less.IH less.prems(2) by blast
+    qed
+    with BabTy_Record show ?thesis by simp
+  next
+    case (BabTy_Array loc elemTy dims)
+    from less.prems(1) BabTy_Array have elem_wk: "is_well_kinded env elemTy"
+      and dims_wk: "array_dims_well_kinded dims"
+      by simp_all
+    from BabTy_Array have "bab_type_size elemTy < bab_type_size ty"
+      by simp
+    with elem_wk less.IH less.prems(2) have "is_well_kinded ?extEnv elemTy"
+      by blast
+    with dims_wk BabTy_Array show ?thesis by simp
+  qed simp_all
+qed
+
+
+(* Definition: all types in the range of a substitution are well-kinded *)
+definition subst_types_well_kinded :: "BabTyEnv \<Rightarrow> (string, BabType) fmap \<Rightarrow> bool" where
+  "subst_types_well_kinded env subst \<equiv>
+    \<forall>name ty. fmlookup subst name = Some ty \<longrightarrow> is_well_kinded env ty"
+
+(* Convenient form for substitutions built from zip *)
+lemma subst_types_well_kinded_from_zip:
+  assumes "list_all (is_well_kinded env) tys"
+  shows "subst_types_well_kinded env (fmap_of_list (zip names tys))"
+  unfolding subst_types_well_kinded_def
+proof (intro allI impI)
+  fix name ty
+  assume "fmlookup (fmap_of_list (zip names tys)) name = Some ty"
+  then have "(name, ty) \<in> set (zip names tys)"
+    by (metis fmap_of_list.rep_eq map_of_SomeD)
+  then have "ty \<in> set tys"
+    by (meson set_zip_rightD)
+  with assms show "is_well_kinded env ty"
+    by (simp add: list_all_iff)
+qed
+
+
+(* Well-kindedness after substitution across environment extension.
+   If ty is well-kinded in env extended with extra type variables (that are not also datatype names),
+   and the substitution covers those extra type variables (i.e., extra \<subseteq> fmdom subst),
+   and all types in the range of subst are well-kinded in the original env,
+   then the result is well-kinded in env. *)
+lemma is_well_kinded_substitute_across_ext:
+  assumes "is_well_kinded (env \<lparr> TE_TypeVars := TE_TypeVars env |\<union>| extra \<rparr>) ty"
+      and "extra |\<inter>| fmdom (TE_Datatypes env) = {||}"
+      and "extra |\<subseteq>| fmdom subst"
+      and "subst_types_well_kinded env subst"
+  shows "is_well_kinded env (substitute_bab_type subst ty)"
+using assms proof (induction ty rule: measure_induct_rule[where f=bab_type_size])
+  case (less ty)
+  let ?extEnv = "env \<lparr> TE_TypeVars := TE_TypeVars env |\<union>| extra \<rparr>"
+  show ?case
+  proof (cases ty)
+    case (BabTy_Name loc name argTypes)
+    show ?thesis
+    proof (cases argTypes)
+      case Nil
+      (* argTypes = [], could be a type variable *)
+      show ?thesis
+      proof (cases "fmlookup subst name")
+        case None
+        (* Not substituted - must be well-kinded in env (not one of the extra tyvars) *)
+        from "less.prems"(1) BabTy_Name Nil have wk_ext: "is_well_kinded ?extEnv (BabTy_Name loc name [])"
+          by simp
+        from wk_ext have "name |\<in>| TE_TypeVars ?extEnv \<or>
+          (\<exists>dtTyVars. fmlookup (TE_Datatypes ?extEnv) name = Some dtTyVars \<and> dtTyVars = [])"
+          by (auto split: if_splits option.splits)
+        hence cases: "name |\<in>| TE_TypeVars env |\<union>| extra \<or>
+          (\<exists>dtTyVars. fmlookup (TE_Datatypes env) name = Some dtTyVars \<and> dtTyVars = [])"
+          by simp
+        (* name is not in extra, because extra \<subseteq> fmdom subst and fmlookup subst name = None *)
+        from None have "name |\<notin>| fmdom subst"
+          by (simp add: fmdom_notI)
+        with "less.prems"(3) have "name |\<notin>| extra"
+          by auto
+        with cases have "name |\<in>| TE_TypeVars env \<or>
+          (\<exists>dtTyVars. fmlookup (TE_Datatypes env) name = Some dtTyVars \<and> dtTyVars = [])"
+          by auto
+        hence "is_well_kinded env (BabTy_Name loc name [])"
+          by (auto split: if_splits option.splits)
+        with None Nil BabTy_Name show ?thesis by simp
+      next
+        case (Some substTy)
+        (* Substituted - substTy is well-kinded in env by subst_types_well_kinded *)
+        from "less.prems"(4) Some have "is_well_kinded env substTy"
+          unfolding subst_types_well_kinded_def by blast
+        with Some Nil BabTy_Name show ?thesis by simp
+      qed
+    next
+      case (Cons a list)
+      (* argTypes non-empty, not a type variable reference, recurse on args *)
+      from "less.prems"(1) BabTy_Name Cons have
+        not_tyvar: "\<not> (name |\<in>| TE_TypeVars ?extEnv)" and
+        dt_lookup: "\<exists>dtTyVars. fmlookup (TE_Datatypes ?extEnv) name = Some dtTyVars \<and>
+                    length (a # list) = length dtTyVars" and
+        args_wk: "list_all (is_well_kinded ?extEnv) (a # list)"
+        by (auto split: if_splits option.splits)
+      from dt_lookup obtain dtTyVars where
+        dt: "fmlookup (TE_Datatypes env) name = Some dtTyVars" and
+        len_eq: "length (a # list) = length dtTyVars"
+        by auto
+      (* name is a datatype, so it's not in extra (by the non-shadowing assumption) *)
+      from dt have "name |\<in>| fmdom (TE_Datatypes env)"
+        by (simp add: fmdomI)
+      with "less.prems"(2) have "name |\<notin>| extra"
+        by auto
+      (* name is not a type variable in env either *)
+      with not_tyvar have not_tyvar_env: "name |\<notin>| TE_TypeVars env"
+        by simp
+      (* By IH, substituted args are well-kinded in env *)
+      have subst_args_wk: "list_all (is_well_kinded env) (map (substitute_bab_type subst) (a # list))"
+      proof -
+        have "\<forall>t \<in> set (a # list). is_well_kinded env (substitute_bab_type subst t)"
+        proof
+          fix t assume t_in: "t \<in> set (a # list)"
+          from t_in BabTy_Name Cons have "bab_type_size t < bab_type_size ty"
+            using bab_type_smaller_than_list bab_type_size.simps(1) plus_1_eq_Suc by presburger
+          moreover from args_wk t_in have "is_well_kinded ?extEnv t"
+            unfolding list.pred_set by blast
+          ultimately show "is_well_kinded env (substitute_bab_type subst t)"
+            using "less.IH" "less.prems"(2) "less.prems"(3) "less.prems"(4) by blast
+        qed
+        thus ?thesis by (simp add: list_all_iff)
+      qed
+      have len_eq': "length (map (substitute_bab_type subst) (a # list)) = length dtTyVars"
+        using len_eq by simp
+      with dt not_tyvar_env len_eq' subst_args_wk BabTy_Name Cons show ?thesis
+        by auto
+    qed
+  next
+    case (BabTy_Bool loc)
+    then show ?thesis by simp
+  next
+    case (BabTy_FiniteInt loc sign bits)
+    then show ?thesis by simp
+  next
+    case (BabTy_MathInt loc)
+    then show ?thesis by simp
+  next
+    case (BabTy_MathReal loc)
+    then show ?thesis by simp
+  next
+    case (BabTy_Tuple loc tys)
+    from "less.prems"(1) BabTy_Tuple have tys_wk: "list_all (is_well_kinded ?extEnv) tys"
+      by simp
+    have "list_all (is_well_kinded env) (map (substitute_bab_type subst) tys)"
+    proof (simp add: list_all_iff, intro ballI)
+      fix t assume t_in: "t \<in> set tys"
+      from t_in BabTy_Tuple have "bab_type_size t < bab_type_size ty"
+        using bab_type_smaller_than_list by simp
+      moreover from tys_wk t_in have "is_well_kinded ?extEnv t"
+        by (simp add: list_all_iff)
+      ultimately show "is_well_kinded env (substitute_bab_type subst t)"
+        using "less.IH" "less.prems"(2) "less.prems"(3) "less.prems"(4) by blast
+    qed
+    with BabTy_Tuple show ?thesis by simp
+  next
+    case (BabTy_Record loc flds)
+    from "less.prems"(1) BabTy_Record have flds_wk: "list_all (is_well_kinded ?extEnv \<circ> snd) flds"
+      by simp
+    have "list_all (is_well_kinded env \<circ> snd) (map (\<lambda>(name, ty). (name, substitute_bab_type subst ty)) flds)"
+    proof -
+      have "\<forall>fld \<in> set flds. is_well_kinded env (substitute_bab_type subst (snd fld))"
+      proof
+        fix fld assume fld_in: "fld \<in> set flds"
+        from fld_in BabTy_Record have "bab_type_size (snd fld) < bab_type_size ty"
+          using bab_type_smaller_than_fieldlist
+          by (metis bab_type_size.simps(7) plus_1_eq_Suc prod.exhaust_sel)
+        moreover from flds_wk fld_in have "is_well_kinded ?extEnv (snd fld)"
+          unfolding list.pred_set by auto
+        ultimately show "is_well_kinded env (substitute_bab_type subst (snd fld))"
+          using "less.IH" "less.prems"(2) "less.prems"(3) "less.prems"(4) by blast
+      qed
+      thus ?thesis by (auto simp: list_all_iff)
+    qed
+    with BabTy_Record show ?thesis by auto
+  next
+    case (BabTy_Array loc elemTy dims)
+    from "less.prems"(1) BabTy_Array have elem_wk: "is_well_kinded ?extEnv elemTy"
+      and dims_wk: "array_dims_well_kinded dims"
+      by simp_all
+    from BabTy_Array have "bab_type_size elemTy < bab_type_size ty"
+      by simp
+    with elem_wk "less.IH" "less.prems"(2) "less.prems"(3) "less.prems"(4)
+    have "is_well_kinded env (substitute_bab_type subst elemTy)"
+      by blast
+    with dims_wk BabTy_Array show ?thesis by simp
+  next
+    case (BabTy_Meta n)
+    then show ?thesis by simp
+  qed
+qed
+
+(* Substitution preserves well-kindedness when all substituted types are well-kinded.
+   This is a corollary of is_well_kinded_substitute_across_ext with extra = {||} *)
+corollary substitute_bab_type_well_kinded:
+  assumes "is_well_kinded env ty"
+      and "subst_types_well_kinded env subst"
+  shows "is_well_kinded env (substitute_bab_type subst ty)"
+proof -
+  (* ty is well-kinded in env, which equals env with empty extension *)
+  have "env \<lparr> TE_TypeVars := TE_TypeVars env |\<union>| {||} \<rparr> = env"
+    by simp
+  with assms(1) have wk_ext: "is_well_kinded (env \<lparr> TE_TypeVars := TE_TypeVars env |\<union>| {||} \<rparr>) ty"
+    by simp
+  (* The conditions for is_well_kinded_substitute_across_ext are trivially satisfied *)
+  have disjoint: "{||} |\<inter>| fmdom (TE_Datatypes env) = {||}"
+    by simp
+  have subset: "{||} |\<subseteq>| fmdom subst"
+    by simp
+  from is_well_kinded_substitute_across_ext[OF wk_ext disjoint subset assms(2)]
+  show ?thesis by simp
+qed
+
 
 end
