isabelle/type_system/TypeEnv.thy
@@ -2,9 +2,10 @@ theory TypeEnv
   imports "../base/BabSyntax" "TypesEqual"
 begin
 
+(* Note: all types contained in the BabTyEnv are fully elaborated *)
+
 record BabTyEnv =
   (* Term-level bindings: variables and constants *)
-  (* Types are kind-correct and all typedefs are resolved *)
   TE_TermVars :: "(string, BabType) fmap"
 
   (* Ghost variables - subset of TE_TermVars keys *)
@@ -14,15 +15,13 @@ record BabTyEnv =
   TE_TypeVars :: "string fset"
 
   (* Function signatures *)
-  (* DeclFuns are valid and have all typedefs resolved *)
   TE_Functions :: "(string, DeclFun) fmap"
 
-  (* Datatype definitions *)
-  (* DeclDatatypes are valid and have all typedefs resolved *)
-  TE_Datatypes :: "(string, DeclDatatype) fmap"
+  (* Datatype type parameters: maps datatype name to list of type variable names *)
+  TE_Datatypes :: "(string, string list) fmap"
 
   (* Data constructors: maps constructor name to (datatype name, num type args, payload type) *)
-  (* This should be consistent with TE_Datatypes *)
+  (* The num type args should be consistent with TE_Datatypes *)
   TE_DataCtors :: "(string, string \<times> nat \<times> BabType option) fmap"
 
 
@@ -49,40 +48,5 @@ fun add_type_var :: "string \<Rightarrow> BabTyEnv \<Rightarrow> BabTyEnv" where
 fun clear_locals :: "BabTyEnv \<Rightarrow> BabTyEnv" where
   "clear_locals env = env \<lparr> TE_TermVars := fmempty, TE_GhostVars := {||}, TE_TypeVars := {||} \<rparr>"
 *)
-
-(* Check if a type is an integer type *)
-fun is_integer_type :: "BabType \<Rightarrow> bool" where
-  "is_integer_type (BabTy_FiniteInt _ _ _) = True"
-| "is_integer_type (BabTy_MathInt _) = True"
-| "is_integer_type _ = False"
-
-(* Check if a type is a signed integer type (signed finite int or MathInt) *)
-fun is_signed_integer_type :: "BabType \<Rightarrow> bool" where
-  "is_signed_integer_type (BabTy_FiniteInt _ Signed _) = True"
-| "is_signed_integer_type (BabTy_MathInt _) = True"
-| "is_signed_integer_type _ = False"
-
-(* Check if a type is a finite integer type *)
-fun is_finite_integer_type :: "BabType \<Rightarrow> bool" where
-  "is_finite_integer_type (BabTy_FiniteInt _ _ _) = True"
-| "is_finite_integer_type _ = False"
-
-(* Check if an array dimension is resolved (not BabDim_Fixed) *)
-fun is_resolved_dimension :: "BabDimension \<Rightarrow> bool" where
-  "is_resolved_dimension (BabDim_Fixed _) = False"
-| "is_resolved_dimension _ = True"
-
-(* Check if a type is a runtime-compatible type (no MathInt/MathReal) *)
-(* Note: Metavariables are considered runtime types, but metavariables should theoretically
-   be removed anyway, post type inference. *)
-fun is_runtime_type :: "BabType \<Rightarrow> bool" where
-  "is_runtime_type (BabTy_MathInt _) = False"
-| "is_runtime_type (BabTy_MathReal _) = False"
-| "is_runtime_type (BabTy_Name _ _ tyArgs) = list_all is_runtime_type tyArgs"
-| "is_runtime_type (BabTy_Tuple _ tys) = list_all is_runtime_type tys"
-| "is_runtime_type (BabTy_Record _ flds) = list_all (is_runtime_type \<circ> snd) flds"
-| "is_runtime_type (BabTy_Array _ ty _) = is_runtime_type ty"
-| "is_runtime_type _ = True"
-
 
 end
