isabelle/type_system/TypeEnvWellFormed.thy
@@ -2,34 +2,78 @@ theory TypeEnvWellFormed
   imports BabKindcheck
 begin
 
+(* All term variable types are well-kinded *)
+definition tyenv_vars_well_kinded :: "BabTyEnv \<Rightarrow> bool" where
+  "tyenv_vars_well_kinded env \<equiv>
+    \<forall>name ty. fmlookup (TE_TermVars env) name = Some ty \<longrightarrow> is_well_kinded env ty"
+
 (* All term variable types are ground (no metavariables) *)
 definition tyenv_vars_ground :: "BabTyEnv \<Rightarrow> bool" where
   "tyenv_vars_ground env \<equiv>
     \<forall>name ty. fmlookup (TE_TermVars env) name = Some ty \<longrightarrow> is_ground ty"
 
-(* All non-ghost variables have runtime types *)
+(* All non-ghost term variable types are runtime types *)
 definition tyenv_vars_runtime :: "BabTyEnv \<Rightarrow> bool" where
   "tyenv_vars_runtime env \<equiv>
     \<forall>name ty. fmlookup (TE_TermVars env) name = Some ty
               \<and> name |\<notin>| TE_GhostVars env
               \<longrightarrow> is_runtime_type ty"
 
-(* All term variable types are well-kinded *)
-definition tyenv_vars_well_kinded :: "BabTyEnv \<Rightarrow> bool" where
-  "tyenv_vars_well_kinded env \<equiv>
-    \<forall>name ty. fmlookup (TE_TermVars env) name = Some ty \<longrightarrow> is_well_kinded env ty"
-
 (* Data constructors are consistent with datatypes:
    for each ctor in TE_DataCtors mapping to (dtName, numTyArgs, payload),
-   dtName must be in TE_Datatypes with matching type argument count,
+   dtName must be in TE_Datatypes with a type variable list of matching length,
    and dtName must not be a type variable *)
 definition tyenv_ctors_consistent :: "BabTyEnv \<Rightarrow> bool" where
   "tyenv_ctors_consistent env \<equiv>
     \<forall>ctorName dtName numTyArgs payload.
       fmlookup (TE_DataCtors env) ctorName = Some (dtName, numTyArgs, payload) \<longrightarrow>
-      (\<exists>dt. fmlookup (TE_Datatypes env) dtName = Some dt \<and>
-            length (DD_TyArgs dt) = numTyArgs \<and>
-            dtName |\<notin>| TE_TypeVars env)"
+      (\<exists>tyVars. fmlookup (TE_Datatypes env) dtName = Some tyVars \<and>
+                length tyVars = numTyArgs \<and>
+                dtName |\<notin>| TE_TypeVars env)"
+
+(* All data constructor payload types are well-kinded *)
+definition tyenv_payloads_well_kinded :: "BabTyEnv \<Rightarrow> bool" where
+  "tyenv_payloads_well_kinded env \<equiv>
+    \<forall>ctorName dtName numTyArgs payloadTy.
+      fmlookup (TE_DataCtors env) ctorName = Some (dtName, numTyArgs, Some payloadTy) \<longrightarrow>
+      is_well_kinded env payloadTy"
+
+(* All datatype type variable lists are distinct *)
+definition tyenv_datatypes_distinct :: "BabTyEnv \<Rightarrow> bool" where
+  "tyenv_datatypes_distinct env \<equiv>
+    \<forall>dtName tyVars.
+      fmlookup (TE_Datatypes env) dtName = Some tyVars \<longrightarrow>
+      distinct tyVars"
+
+(* Helper: environment extended with type variables from a function declaration *)
+definition env_with_tyvars :: "BabTyEnv \<Rightarrow> string list \<Rightarrow> BabTyEnv" where
+  "env_with_tyvars env tyVars \<equiv>
+    env \<lparr> TE_TypeVars := TE_TypeVars env |\<union>| fset_of_list tyVars \<rparr>"
+
+(* Function declarations are well-formed:
+   - Function type variables don't shadow datatype names
+   - All argument types are ground and well-kinded (in env extended with function's type variables)
+   - Return type (if present) is ground and well-kinded (in env extended with function's type variables)
+   - For non-ghost functions, argument types and return type must be runtime types *)
+definition tyenv_functions_well_formed :: "BabTyEnv \<Rightarrow> bool" where
+  "tyenv_functions_well_formed env \<equiv>
+    \<forall>fnName funDecl.
+      fmlookup (TE_Functions env) fnName = Some funDecl \<longrightarrow>
+      (let extEnv = env_with_tyvars env (DF_TyArgs funDecl) in
+        \<comment> \<open>Function type variables don't shadow datatype names\<close>
+        fset_of_list (DF_TyArgs funDecl) |\<inter>| fmdom (TE_Datatypes env) = {||} \<and>
+        \<comment> \<open>All argument types are ground and well-kinded\<close>
+        list_all (\<lambda>(_, _, ty). is_ground ty \<and> is_well_kinded extEnv ty) (DF_TmArgs funDecl) \<and>
+        \<comment> \<open>Return type (if present) is ground and well-kinded\<close>
+        (case DF_ReturnType funDecl of
+          None \<Rightarrow> True
+        | Some retTy \<Rightarrow> is_ground retTy \<and> is_well_kinded extEnv retTy) \<and>
+        \<comment> \<open>For non-ghost functions, types must be runtime types\<close>
+        (DF_Ghost funDecl = NotGhost \<longrightarrow>
+          list_all (\<lambda>(_, _, ty). is_runtime_type ty) (DF_TmArgs funDecl) \<and>
+          (case DF_ReturnType funDecl of
+            None \<Rightarrow> True
+          | Some retTy \<Rightarrow> is_runtime_type retTy)))"
 
 (* A type environment is well-formed if all the above conditions hold *)
 definition tyenv_well_formed :: "BabTyEnv \<Rightarrow> bool" where
@@ -37,6 +81,9 @@ definition tyenv_well_formed :: "BabTyEnv \<Rightarrow> bool" where
     tyenv_vars_ground env \<and>
     tyenv_vars_runtime env \<and>
     tyenv_vars_well_kinded env \<and>
-    tyenv_ctors_consistent env"
+    tyenv_ctors_consistent env \<and>
+    tyenv_payloads_well_kinded env \<and>
+    tyenv_datatypes_distinct env \<and>
+    tyenv_functions_well_formed env"
 
 end
