isabelle/interpreter/TypeSoundness.thy
@@ -1,0 +1,726 @@
+theory TypeSoundness
+  imports "ValueTyping"
+begin
+
+(*-----------------------------------------------------------------------------*)
+(* Definition of soundness for interpreter results *)
+(*-----------------------------------------------------------------------------*)
+
+(* Type soundness means that evaluating a well-typed term will always either:
+    - Succeed with a value of the correct type
+    - Fail with a RuntimeError
+    - Run out of fuel
+   It will never:
+    - Succeed with a value that doesn't match the type of the term
+    - Fail with a TypeError
+*)
+
+definition is_sound_result :: "BabTyEnv \<Rightarrow> BabType \<Rightarrow> BabValue BabInterpResult \<Rightarrow> bool" where
+  "is_sound_result env ty result \<equiv>
+    (case result of
+       BIR_Success val \<Rightarrow> value_has_type env val ty
+     | BIR_TypeError \<Rightarrow> False
+     | BIR_RuntimeError \<Rightarrow> True
+     | BIR_InsufficientFuel \<Rightarrow> True)"
+
+lemma is_sound_result_Success [simp]:
+  "is_sound_result env ty (BIR_Success val) = value_has_type env val ty"
+  unfolding is_sound_result_def by simp
+
+lemma is_sound_result_TypeError [simp]:
+  "\<not> is_sound_result env ty BIR_TypeError"
+  unfolding is_sound_result_def by simp
+
+lemma is_sound_result_RuntimeError [simp]:
+  "is_sound_result env ty BIR_RuntimeError"
+  unfolding is_sound_result_def by simp
+
+lemma is_sound_result_InsufficientFuel [simp]:
+  "is_sound_result env ty BIR_InsufficientFuel"
+  unfolding is_sound_result_def by simp
+
+
+(*-----------------------------------------------------------------------------*)
+(* Helper lemmas for type soundness *)
+(*-----------------------------------------------------------------------------*)
+
+(* Property of int_complement *)
+lemma int_complement_fits:
+  assumes "int_fits sign bits i"
+  shows "int_fits sign bits (int_complement sign bits i)"
+  using assms by (cases sign; cases bits; auto)
+
+(* Type soundness for Cast *)
+lemma type_soundness_cast:
+  assumes state_env: "state_matches_env state env"
+    and wf_env: "tyenv_well_formed env"
+    and IH: "\<And>tm' ty'. bab_term_type env NotGhost tm' = Some ty' \<Longrightarrow>
+                        is_sound_result env ty' (interp_bab_term fuel state tm')"
+    and typing: "bab_term_type env NotGhost (BabTm_Cast loc target_ty operand) = Some ty"
+  shows "is_sound_result env ty (interp_bab_term (Suc fuel) state (BabTm_Cast loc target_ty operand))"
+proof -
+  (* Extract facts from typing *)
+  from typing obtain operand_ty where
+    operand_typing: "bab_term_type env NotGhost operand = Some operand_ty"
+    and operand_is_int: "is_integer_type operand_ty"
+    and target_is_int: "is_integer_type target_ty"
+    and ty_eq: "ty = target_ty"
+    by (auto split: option.splits if_splits)
+
+  (* Apply IH to operand *)
+  from IH[OF operand_typing]
+  have operand_sound: "is_sound_result env operand_ty (interp_bab_term fuel state operand)"
+    by simp
+
+  (* Case split on operand result *)
+  show ?thesis
+  proof (cases "interp_bab_term fuel state operand")
+    case (BIR_Success operand_val)
+    (* Operand succeeded - extract type information *)
+    from operand_sound BIR_Success
+    have operand_typed: "value_has_type env operand_val operand_ty"
+      by simp
+
+    (* Since operand has an integer type, value must be BV_FiniteInt or BV_MathInt *)
+    from operand_typed operand_is_int
+    consider (FiniteInt) src_sign src_bits i where "operand_val = BV_FiniteInt src_sign src_bits i"
+           | (MathInt) i where "operand_val = BV_MathInt i"
+      using value_has_integer_type_cases by blast
+    then show ?thesis
+    proof cases
+      case (FiniteInt src_sign src_bits i)
+      (* Target type must be a finite integer type (from is_integer_type + runtime type check) *)
+      from target_is_int obtain loc' tgt_sign tgt_bits where
+        target_ty_def: "target_ty = BabTy_FiniteInt loc' tgt_sign tgt_bits"
+        using BIR_Success FiniteInt is_integer_type.elims(2) operand_typing typing by fastforce
+
+      (* Case split on whether cast succeeds *)
+      show ?thesis
+      proof (cases "int_fits tgt_sign tgt_bits i")
+        case True
+        (* Cast succeeds - value has correct type *)
+        from BIR_Success FiniteInt target_ty_def True
+        have "interp_bab_term (Suc fuel) state (BabTm_Cast loc target_ty operand) =
+              BIR_Success (BV_FiniteInt tgt_sign tgt_bits i)"
+          by auto
+        with ty_eq target_ty_def True show ?thesis by auto
+      next
+        case False
+        (* Cast fails with RuntimeError *)
+        from BIR_Success FiniteInt target_ty_def False
+        have "interp_bab_term (Suc fuel) state (BabTm_Cast loc target_ty operand) = BIR_RuntimeError"
+          by auto
+        thus ?thesis by simp
+      qed
+    next
+      case (MathInt i)
+      (* MathInt is not a runtime type, so this contradicts bab_term_type_runtime_invariant *)
+      from operand_typed MathInt obtain loc' where "operand_ty = BabTy_MathInt loc'"
+        by (cases operand_ty; auto)
+      then have "\<not> is_runtime_type operand_ty"
+        by simp
+      thus ?thesis
+        using bab_term_type_runtime_invariant operand_typing wf_env by auto
+    qed
+  next
+    case BIR_TypeError
+    (* Operand returned TypeError - contradicts soundness of operand *)
+    from operand_sound BIR_TypeError show ?thesis by simp
+  next
+    case BIR_RuntimeError
+    from BIR_RuntimeError show ?thesis by simp
+  next
+    case BIR_InsufficientFuel
+    from BIR_InsufficientFuel show ?thesis by simp
+  qed
+qed
+
+(* Type soundness for if-then-else *)
+lemma type_soundness_if:
+  assumes state_env: "state_matches_env state env"
+    and wf_env: "tyenv_well_formed env"
+    and IH: "\<And>tm' ty'. bab_term_type env NotGhost tm' = Some ty' \<Longrightarrow>
+                        is_sound_result env ty' (interp_bab_term fuel state tm')"
+    and typing: "bab_term_type env NotGhost (BabTm_If loc cond thenTm elseTm) = Some ty"
+  shows "is_sound_result env ty (interp_bab_term (Suc fuel) state (BabTm_If loc cond thenTm elseTm))"
+proof -
+  (* Extract facts from typing - the typechecker only succeeds if all these hold *)
+  obtain cond_ty where cond_typing: "bab_term_type env NotGhost cond = Some cond_ty"
+    using typing by (auto split: option.splits)
+  obtain bloc where cond_is_bool: "cond_ty = BabTy_Bool bloc"
+    using typing cond_typing by (auto split: BabType.splits)
+  obtain then_ty else_ty where
+    then_typing: "bab_term_type env NotGhost thenTm = Some then_ty"
+    and else_typing: "bab_term_type env NotGhost elseTm = Some else_ty"
+    using typing cond_typing cond_is_bool by (auto split: option.splits)
+  have types_match: "types_equal then_ty else_ty"
+    using typing cond_typing cond_is_bool then_typing else_typing by (auto split: if_splits)
+  have ty_eq: "ty = then_ty"
+    using typing cond_typing cond_is_bool then_typing else_typing types_match by auto
+
+  (* Apply IH to subterms *)
+  from IH[OF cond_typing] have cond_sound:
+    "is_sound_result env cond_ty (interp_bab_term fuel state cond)" .
+  from IH[OF then_typing] have then_sound:
+    "is_sound_result env then_ty (interp_bab_term fuel state thenTm)" .
+  from IH[OF else_typing] have else_sound:
+    "is_sound_result env else_ty (interp_bab_term fuel state elseTm)" .
+
+  (* Case split on condition result *)
+  show ?thesis
+  proof (cases "interp_bab_term fuel state cond")
+    case (BIR_Success cond_val)
+    from cond_sound BIR_Success have cond_typed: "value_has_type env cond_val cond_ty"
+      by simp
+
+    (* Condition must be a bool *)
+    from cond_is_bool cond_typed obtain b where cond_val_def: "cond_val = BV_Bool b"
+      using value_has_type_Bool by blast
+
+    (* Case split on boolean value *)
+    show ?thesis
+    proof (cases b)
+      case True
+      (* Condition is true, evaluate then branch *)
+      from BIR_Success cond_val_def True
+      have interp_eq: "interp_bab_term (Suc fuel) state (BabTm_If loc cond thenTm elseTm) =
+                       interp_bab_term fuel state thenTm"
+        by auto
+      from then_sound ty_eq interp_eq show ?thesis by simp
+    next
+      case False
+      (* Condition is false, evaluate else branch *)
+      from BIR_Success cond_val_def False
+      have interp_eq: "interp_bab_term (Suc fuel) state (BabTm_If loc cond thenTm elseTm) =
+                       interp_bab_term fuel state elseTm"
+        by auto
+
+      (* Need to show result has type then_ty, but else branch has type else_ty *)
+      show ?thesis
+      proof (cases "interp_bab_term fuel state elseTm")
+        case (BIR_Success val)
+        from else_sound BIR_Success have val_has_else_ty: "value_has_type env val else_ty"
+          by simp
+
+        (* Use types_equal to convert from else_ty to then_ty *)
+        from types_match have else_ty_eq_then_ty: "types_equal else_ty then_ty"
+          using types_equal_symmetric by metis
+
+        (* else_ty is well-kinded because bab_term_type produces well-kinded types *)
+        from else_typing wf_env have else_ty_wk: "is_well_kinded env else_ty"
+          by (rule bab_term_type_well_kinded)
+
+        (* Apply value_has_type_types_equal *)
+        from val_has_else_ty else_ty_eq_then_ty wf_env else_ty_wk
+        have "value_has_type env val then_ty"
+          by (rule value_has_type_types_equal)
+        with ty_eq interp_eq BIR_Success show ?thesis by simp
+      next
+        case BIR_TypeError
+        from else_sound BIR_TypeError show ?thesis by simp
+      next
+        case BIR_RuntimeError
+        from interp_eq BIR_RuntimeError show ?thesis by simp
+      next
+        case BIR_InsufficientFuel
+        from interp_eq BIR_InsufficientFuel show ?thesis by simp
+      qed
+    qed
+  next
+    case BIR_TypeError
+    from cond_sound BIR_TypeError show ?thesis by simp
+  next
+    case BIR_RuntimeError
+    from BIR_RuntimeError show ?thesis by simp
+  next
+    case BIR_InsufficientFuel
+    from BIR_InsufficientFuel show ?thesis by simp
+  qed
+qed
+
+(* Type soundness for unary operators *)
+lemma type_soundness_unop:
+  assumes state_env: "state_matches_env state env"
+    and wf_env: "tyenv_well_formed env"
+    and IH: "\<And>tm' ty'. bab_term_type env NotGhost tm' = Some ty' \<Longrightarrow>
+                        is_sound_result env ty' (interp_bab_term fuel state tm')"
+    and typing: "bab_term_type env NotGhost (BabTm_Unop loc unop operand) = Some ty"
+  shows "is_sound_result env ty (interp_bab_term (Suc fuel) state (BabTm_Unop loc unop operand))"
+proof (cases unop)
+  case BabUnop_Negate
+  (* Negate: operand must be signed integer, result has same type *)
+  from BabUnop_Negate typing obtain operand_ty where
+    operand_typing: "bab_term_type env NotGhost operand = Some operand_ty"
+    and is_int: "is_integer_type operand_ty"
+    and ty_eq: "ty = operand_ty"
+    by (auto simp: signed_integer_type_is_integer_type split: option.splits if_splits)
+
+  from IH[OF operand_typing] have operand_sound:
+    "is_sound_result env operand_ty (interp_bab_term fuel state operand)" .
+
+  show ?thesis
+  proof (cases "interp_bab_term fuel state operand")
+    case (BIR_Success operand_val)
+    from operand_sound BIR_Success have operand_typed: "value_has_type env operand_val operand_ty"
+      by simp
+
+    (* Since operand has an integer type, value must be BV_FiniteInt or BV_MathInt *)
+    from operand_typed is_int
+    consider (FiniteInt) sign bits i where "operand_val = BV_FiniteInt sign bits i"
+           | (MathInt) i where "operand_val = BV_MathInt i"
+      using value_has_integer_type_cases by blast
+    then show ?thesis
+    proof cases
+      case (FiniteInt sign bits i)
+      (* Since operand_ty is an integer type and value has that type, extract type info *)
+      from operand_typed FiniteInt obtain loc' sign' bits' where operand_ty_def:
+        "operand_ty = BabTy_FiniteInt loc' sign' bits'"
+        and sign_eq: "sign = sign'" and bits_eq: "bits = bits'"
+        and fits: "int_fits sign bits i"
+        by (cases operand_ty; auto)
+
+      show ?thesis
+      proof (cases "int_fits sign bits (-i)")
+        case True
+        (* Negation succeeds *)
+        from BabUnop_Negate BIR_Success FiniteInt True
+        have "interp_bab_term (Suc fuel) state (BabTm_Unop loc unop operand) =
+              BIR_Success (BV_FiniteInt sign bits (-i))"
+          by auto
+        with ty_eq operand_ty_def sign_eq bits_eq True show ?thesis by auto
+      next
+        case False
+        (* Negation overflows - RuntimeError *)
+        from BabUnop_Negate BIR_Success FiniteInt False
+        have "interp_bab_term (Suc fuel) state (BabTm_Unop loc unop operand) = BIR_RuntimeError"
+          by auto
+        thus ?thesis by simp
+      qed
+    next
+      case (MathInt i)
+      (* MathInt is not a runtime type - contradiction *)
+      from operand_typed MathInt obtain loc' where "operand_ty = BabTy_MathInt loc'"
+        by (cases operand_ty; auto)
+      then have "\<not> is_runtime_type operand_ty"
+        by simp
+      thus ?thesis
+        using bab_term_type_runtime_invariant operand_typing wf_env by auto
+    qed
+  next
+    case BIR_TypeError
+    from operand_sound BIR_TypeError show ?thesis by simp
+  next
+    case BIR_RuntimeError
+    from BabUnop_Negate BIR_RuntimeError show ?thesis by simp
+  next
+    case BIR_InsufficientFuel
+    from BabUnop_Negate BIR_InsufficientFuel show ?thesis by simp
+  qed
+next
+  case BabUnop_Complement
+  (* Complement: operand must be finite integer, result has same type *)
+  from BabUnop_Complement typing obtain operand_ty where
+    operand_typing: "bab_term_type env NotGhost operand = Some operand_ty"
+    and is_int: "is_integer_type operand_ty"
+    and ty_eq: "ty = operand_ty"
+    by (auto simp: finite_integer_type_is_integer_type split: option.splits if_splits)
+
+  from IH[OF operand_typing] have operand_sound:
+    "is_sound_result env operand_ty (interp_bab_term fuel state operand)" .
+
+  show ?thesis
+  proof (cases "interp_bab_term fuel state operand")
+    case (BIR_Success operand_val)
+    from operand_sound BIR_Success have operand_typed: "value_has_type env operand_val operand_ty"
+      by simp
+
+    (* Since operand has an integer type, value must be BV_FiniteInt or BV_MathInt *)
+    from operand_typed is_int
+    consider (FiniteInt) sign bits i where "operand_val = BV_FiniteInt sign bits i"
+           | (MathInt) i where "operand_val = BV_MathInt i"
+      using value_has_integer_type_cases by blast
+    then show ?thesis
+    proof cases
+      case (FiniteInt sign bits i)
+      from operand_typed FiniteInt obtain loc' sign' bits' where operand_ty_def:
+        "operand_ty = BabTy_FiniteInt loc' sign' bits'"
+        and sign_eq: "sign = sign'" and bits_eq: "bits = bits'"
+        and fits: "int_fits sign bits i"
+        by (cases operand_ty; auto)
+
+      (* Complement always succeeds and fits *)
+      from BabUnop_Complement BIR_Success FiniteInt
+      have interp_eq: "interp_bab_term (Suc fuel) state (BabTm_Unop loc unop operand) =
+            BIR_Success (BV_FiniteInt sign bits (int_complement sign bits i))"
+        by auto
+
+      have comp_fits: "int_fits sign bits (int_complement sign bits i)"
+        using fits by (rule int_complement_fits)
+
+      from interp_eq ty_eq operand_ty_def sign_eq bits_eq comp_fits
+      show ?thesis by auto
+    next
+      case (MathInt i)
+      (* MathInt is not a runtime type - contradiction *)
+      from operand_typed MathInt obtain loc' where "operand_ty = BabTy_MathInt loc'"
+        by (cases operand_ty; auto)
+      then have "\<not> is_runtime_type operand_ty"
+        by simp
+      thus ?thesis
+        using bab_term_type_runtime_invariant operand_typing wf_env by auto
+    qed
+  next
+    case BIR_TypeError
+    from operand_sound BIR_TypeError show ?thesis by simp
+  next
+    case BIR_RuntimeError
+    from BabUnop_Complement BIR_RuntimeError show ?thesis by simp
+  next
+    case BIR_InsufficientFuel
+    from BabUnop_Complement BIR_InsufficientFuel show ?thesis by simp
+  qed
+next
+  case BabUnop_Not
+  (* Not: operand must be bool, result is bool *)
+  from BabUnop_Not typing obtain operand_ty bloc where
+    operand_typing: "bab_term_type env NotGhost operand = Some operand_ty"
+    and operand_is_bool: "operand_ty = BabTy_Bool bloc"
+    and ty_eq: "ty = operand_ty"
+    by (auto split: option.splits BabType.splits)
+
+  from IH[OF operand_typing] have operand_sound:
+    "is_sound_result env operand_ty (interp_bab_term fuel state operand)" .
+
+  show ?thesis
+  proof (cases "interp_bab_term fuel state operand")
+    case (BIR_Success operand_val)
+    from operand_sound BIR_Success have operand_typed: "value_has_type env operand_val operand_ty"
+      by simp
+
+    from operand_is_bool operand_typed obtain b where operand_val_def: "operand_val = BV_Bool b"
+      using value_has_type_Bool by blast
+
+    from BabUnop_Not BIR_Success operand_val_def
+    have "interp_bab_term (Suc fuel) state (BabTm_Unop loc unop operand) = BIR_Success (BV_Bool (\<not>b))"
+      by auto
+    with ty_eq operand_is_bool show ?thesis by auto
+  next
+    case BIR_TypeError
+    from operand_sound BIR_TypeError show ?thesis by simp
+  next
+    case BIR_RuntimeError
+    from BabUnop_Not BIR_RuntimeError show ?thesis by simp
+  next
+    case BIR_InsufficientFuel
+    from BabUnop_Not BIR_InsufficientFuel show ?thesis by simp
+  qed
+qed
+
+
+(* Soundness of exec_function_call - assumed for now, to be proved later
+   together with interp_bab_term soundness via mutual induction *)
+lemma exec_function_call_sound:
+  assumes state_env: "state_matches_env state env"
+    and wf_env: "tyenv_well_formed env"
+    and typing: "bab_term_type env NotGhost (BabTm_Call loc fnTm argTms) = Some ty"
+  shows "case exec_function_call fuel state (BabTm_Call loc fnTm argTms) of
+           BIR_Success (_, Some retVal) \<Rightarrow> value_has_type env retVal ty
+         | BIR_Success (_, None) \<Rightarrow> False  \<comment> \<open>Should have return value since ty exists\<close>
+         | BIR_TypeError \<Rightarrow> False
+         | BIR_RuntimeError \<Rightarrow> True
+         | BIR_InsufficientFuel \<Rightarrow> True"
+  sorry
+
+(* Type soundness for function calls *)
+lemma type_soundness_call:
+  assumes state_env: "state_matches_env state env"
+    and wf_env: "tyenv_well_formed env"
+    and IH: "\<And>tm' ty'. bab_term_type env NotGhost tm' = Some ty' \<Longrightarrow>
+                        is_sound_result env ty' (interp_bab_term fuel state tm')"
+    and typing: "bab_term_type env NotGhost (BabTm_Call loc fnTm argTms) = Some ty"
+  shows "is_sound_result env ty (interp_bab_term (Suc fuel) state (BabTm_Call loc fnTm argTms))"
+proof -
+  (* Extract function name and type args from fnTm *)
+  from typing obtain fnLoc fnName tyArgs where
+    fnTm_eq: "fnTm = BabTm_Name fnLoc fnName tyArgs"
+    by (cases fnTm) (auto split: option.splits)
+
+  (* Get function declaration from type environment *)
+  from typing fnTm_eq obtain funDecl where
+    fn_lookup_env: "fmlookup (TE_Functions env) fnName = Some funDecl"
+    by (auto split: option.splits)
+
+  (* Function lookup in state equals function lookup in env *)
+  have fn_lookup_state: "fmlookup (BS_Functions state) fnName = Some funDecl"
+    using function_lookup_eq[OF state_env] fn_lookup_env by simp
+
+  (* Extract conditions from typing *)
+  from typing fnTm_eq fn_lookup_env have
+    not_impure: "\<not> DF_Impure funDecl" and
+    no_ref_args: "\<not> list_ex (\<lambda>(_, vr, _). vr = Ref) (DF_TmArgs funDecl)"
+    by (auto split: option.splits if_splits)
+
+  (* Show is_pure_fun_term state fnTm *)
+  have is_pure: "is_pure_fun_term state fnTm"
+    using fnTm_eq fn_lookup_state no_ref_args not_impure
+    by simp
+
+  (* The interpreter calls exec_function_call when is_pure_fun_term holds *)
+  have interp_eq: "interp_bab_term (Suc fuel) state (BabTm_Call loc fnTm argTms) =
+    (case exec_function_call fuel state (BabTm_Call loc fnTm argTms) of
+       BIR_Success (_, Some retVal) \<Rightarrow> BIR_Success retVal
+     | BIR_Success (_, None) \<Rightarrow> BIR_TypeError
+     | err \<Rightarrow> convert_error err)"
+    using is_pure by simp
+
+  (* Use exec_function_call_sound *)
+  from exec_function_call_sound[OF state_env wf_env typing]
+  have call_sound: "case exec_function_call fuel state (BabTm_Call loc fnTm argTms) of
+           BIR_Success (_, Some retVal) \<Rightarrow> value_has_type env retVal ty
+         | BIR_Success (_, None) \<Rightarrow> False
+         | BIR_TypeError \<Rightarrow> False
+         | BIR_RuntimeError \<Rightarrow> True
+         | BIR_InsufficientFuel \<Rightarrow> True" .
+
+  (* Case split on the result of exec_function_call *)
+  show ?thesis
+  proof (cases "exec_function_call fuel state (BabTm_Call loc fnTm argTms)")
+    case (BIR_Success result)
+    obtain newState maybeRetVal where result_eq: "result = (newState, maybeRetVal)"
+      by (cases result) auto
+    show ?thesis
+    proof (cases maybeRetVal)
+      case None
+      (* This case contradicts call_sound *)
+      from call_sound BIR_Success result_eq None have False by simp
+      thus ?thesis by simp
+    next
+      case (Some retVal)
+      from call_sound BIR_Success result_eq Some have "value_has_type env retVal ty"
+        by simp
+      with interp_eq BIR_Success result_eq Some show ?thesis
+        by simp
+    qed
+  next
+    case BIR_TypeError
+    (* This case contradicts call_sound *)
+    from call_sound BIR_TypeError have False by simp
+    thus ?thesis by simp
+  next
+    case BIR_RuntimeError
+    from interp_eq BIR_RuntimeError show ?thesis by simp
+  next
+    case BIR_InsufficientFuel
+    from interp_eq BIR_InsufficientFuel show ?thesis by simp
+  qed
+qed
+
+
+(*-----------------------------------------------------------------------------*)
+(* Main type soundness theorem *)
+(*-----------------------------------------------------------------------------*)
+
+theorem type_soundness:
+  fixes fuel :: nat
+    and state :: "'w BabState"
+    and env :: BabTyEnv
+  assumes state_env: "state_matches_env state env"
+      and wf_env: "tyenv_well_formed env"
+  shows
+    "\<forall>tm ty.
+       bab_term_type env NotGhost tm = Some ty \<longrightarrow>
+       is_sound_result env ty (interp_bab_term fuel state tm)"
+using assms
+proof (induction fuel arbitrary: state env)
+  case 0
+  (* Base case: fuel = 0 means BIR_InsufficientFuel *)
+  then show ?case by auto
+next
+  case (Suc fuel)
+  (* Inductive case: we have IH for fuel, proving for (Suc fuel) *)
+  show ?case
+  proof (intro allI impI)
+    fix tm ty
+    assume typing: "bab_term_type env NotGhost tm = Some ty"
+
+    (* IH in a more convenient form *)
+    have IH: "\<And>tm' ty'. bab_term_type env NotGhost tm' = Some ty' \<Longrightarrow>
+                        is_sound_result env ty' (interp_bab_term fuel state tm')"
+      using Suc.IH Suc.prems by blast
+
+    (* Case split on the structure of tm *)
+    show "is_sound_result env ty (interp_bab_term (Suc fuel) state tm)"
+    proof (cases tm)
+      case (BabTm_Literal loc lit)
+      (* Case: term is a literal *)
+      then show ?thesis
+      proof (cases lit)
+        case (BabLit_Bool b)
+        (* Bool literal case *)
+        from BabTm_Literal BabLit_Bool typing show ?thesis
+          by (auto split: BabType.splits)
+      next
+        case (BabLit_Int i)
+        (* Int literal case *)
+        from BabTm_Literal BabLit_Int typing show ?thesis
+          by (auto split: if_splits BabType.splits Signedness.splits IntBits.splits)
+      next
+        case (BabLit_String s)
+        (* String literal - TODO *)
+        from BabTm_Literal BabLit_String typing show ?thesis
+          sorry
+      next
+        case (BabLit_Array tms)
+        (* Array literal - TODO *)
+        from BabTm_Literal BabLit_Array typing show ?thesis
+          sorry
+      qed
+    next
+      case (BabTm_Cast loc target_ty operand)
+      (* Cast case - use helper lemma *)
+      from type_soundness_cast[OF Suc.prems(1) Suc.prems(2) IH] BabTm_Cast typing
+      show ?thesis by simp
+    next
+      case (BabTm_Unop loc unop operand)
+      (* Unary operator case - use helper lemma *)
+      from type_soundness_unop[OF Suc.prems(1) Suc.prems(2) IH] BabTm_Unop typing
+      show ?thesis by simp
+    next
+      case (BabTm_Binop loc tm1 ops)
+      (* Binary operator case - TODO *)
+      from BabTm_Binop typing show ?thesis
+        sorry
+    next
+      case (BabTm_If loc cond thenTm elseTm)
+      (* If-then-else case - use helper lemma *)
+      from type_soundness_if[OF Suc.prems(1) Suc.prems(2) IH] BabTm_If typing
+      show ?thesis by simp
+    next
+      case (BabTm_Let loc name bindTm bodyTm)
+      (* Let binding case - TODO *)
+      from BabTm_Let typing show ?thesis
+        sorry
+    next
+      case (BabTm_Quantifier loc quant tyVars vars body)
+      (* Quantifier case - TODO: bab_term_type not implemented for quantifiers yet *)
+      from BabTm_Quantifier typing show ?thesis
+        sorry
+    next
+      case (BabTm_Name loc name tyArgs)
+      (* Variable/constant reference *)
+      from BabTm_Name typing have ty_lookup:
+        "fmlookup (TE_TermVars env) name = Some ty \<and> tyArgs = [] \<and> name |\<notin>| TE_GhostVars env
+         \<or> (\<exists>dtName numTyArgs. fmlookup (TE_DataCtors env) name = Some (dtName, numTyArgs, None) \<and>
+              length tyArgs = numTyArgs \<and> ty = BabTy_Name loc dtName tyArgs)"
+        by (auto split: option.splits if_splits prod.splits)
+      show ?thesis
+      proof (cases "fmlookup (TE_TermVars env) name")
+        case (Some varTy)
+        with ty_lookup have ty_eq: "ty = varTy"
+          by (smt (verit, ccfv_threshold) BabTm_Name bab_term_type.simps(3) option.distinct(1)
+              option.inject option.simps(5) typing)
+        from Suc.prems have vars_wt: "vars_have_correct_types state env"
+          unfolding state_matches_env_def by simp
+        from vars_wt Some have var_typed: "term_var_in_state_with_type state env name varTy"
+          unfolding vars_have_correct_types_def by blast
+        then have var_typed':
+          "(case fmlookup (BS_Locals state) name of
+              Some addr \<Rightarrow> addr < length (BS_Store state) \<and> value_has_type env (BS_Store state ! addr) varTy
+            | None \<Rightarrow>
+              (case fmlookup (BS_RefVars state) name of
+                Some (addr, path) \<Rightarrow> addr < length (BS_Store state) \<and>
+                                     (case get_value_at_path (BS_Store state ! addr) path of
+                                        BIR_Success v \<Rightarrow> value_has_type env v varTy
+                                      | _ \<Rightarrow> False)
+              | None \<Rightarrow>
+                (case fmlookup (BS_Constants state) name of
+                  Some v \<Rightarrow> value_has_type env v varTy
+                | None \<Rightarrow> False)))"
+          unfolding term_var_in_state_with_type by simp
+        with BabTm_Name ty_eq show ?thesis
+          by (auto split: option.splits BabInterpResult.splits simp: is_sound_result_def)
+      next
+        case None
+        (* Data constructor case - name is a nullary data constructor *)
+        from ty_lookup None obtain dtName numTyArgs where
+          ctor_lookup: "fmlookup (TE_DataCtors env) name = Some (dtName, numTyArgs, None)" and
+          len_eq: "length tyArgs = numTyArgs" and
+          ty_eq: "ty = BabTy_Name loc dtName tyArgs"
+          by auto
+        from Suc.prems(1) ctor_lookup have name_in_nullary: "name |\<in>| BS_NullaryCtors state"
+          by (rule nullary_ctor_in_state)
+        (* name is not in locals, refvars, or constants *)
+        from Suc.prems(1) None have not_local: "fmlookup (BS_Locals state) name = None"
+          and not_ref: "fmlookup (BS_RefVars state) name = None"
+          and not_const: "fmlookup (BS_Constants state) name = None"
+          by (auto intro: not_in_env_not_in_state)
+        (* So the interpreter returns BV_Variant name None *)
+        from BabTm_Name not_local not_ref not_const name_in_nullary
+        have interp_result: "interp_bab_term (Suc fuel) state (BabTm_Name loc name tyArgs) =
+                            BIR_Success (BV_Variant name None)"
+          by simp
+        (* Now show the result has the right type *)
+        from ctor_lookup have val_typed: "value_has_type env (BV_Variant name None) (BabTy_Name loc dtName tyArgs)"
+          by simp
+        with interp_result ty_eq show ?thesis
+          by (simp add: BabTm_Name)
+      qed
+    next
+      case (BabTm_Call loc fnTm argTms)
+      (* Function call - use helper lemma *)
+      from type_soundness_call[OF Suc.prems(1) Suc.prems(2) IH] BabTm_Call typing
+      show ?thesis by simp
+    next
+      case (BabTm_Tuple loc tms)
+      (* Tuple construction - TODO *)
+      from BabTm_Tuple typing show ?thesis
+        sorry
+    next
+      case (BabTm_Record loc fields)
+      (* Record construction - TODO *)
+      from BabTm_Record typing show ?thesis
+        sorry
+    next
+      case (BabTm_RecordUpdate loc baseTm updates)
+      (* Record update - TODO *)
+      from BabTm_RecordUpdate typing show ?thesis
+        sorry
+    next
+      case (BabTm_TupleProj loc tm idx)
+      (* Tuple projection - TODO *)
+      from BabTm_TupleProj typing show ?thesis
+        sorry
+    next
+      case (BabTm_RecordProj loc tm field)
+      (* Record projection - TODO *)
+      from BabTm_RecordProj typing show ?thesis
+        sorry
+    next
+      case (BabTm_ArrayProj loc arrTm indices)
+      (* Array projection - TODO *)
+      from BabTm_ArrayProj typing show ?thesis
+        sorry
+    next
+      case (BabTm_Match loc scrutTm arms)
+      (* Match expression - TODO *)
+      from BabTm_Match typing show ?thesis
+        sorry
+    next
+      case (BabTm_Sizeof loc tm)
+      (* Sizeof expression - TODO *)
+      from BabTm_Sizeof typing show ?thesis
+        sorry
+    next
+      case (BabTm_Allocated loc tm)
+      (* Allocated returns None in NotGhost mode, so typing assumption is false *)
+      from BabTm_Allocated typing show ?thesis by simp
+    next
+      case (BabTm_Old loc tm)
+      (* Old - interpreter returns TypeError, but typechecker is still TODO *)
+      from BabTm_Old show ?thesis sorry
+    qed
+  qed
+qed
+
+
+end
