isabelle/type_system/TypeProps.thy
@@ -1,0 +1,122 @@
+theory TypeProps
+  imports "../base/BabSyntax"
+begin
+
+(* Check if a type is an integer type *)
+fun is_integer_type :: "BabType \<Rightarrow> bool" where
+  "is_integer_type (BabTy_FiniteInt _ _ _) = True"
+| "is_integer_type (BabTy_MathInt _) = True"
+| "is_integer_type _ = False"
+
+(* Check if a type is a signed integer type (signed finite int or MathInt) *)
+fun is_signed_integer_type :: "BabType \<Rightarrow> bool" where
+  "is_signed_integer_type (BabTy_FiniteInt _ Signed _) = True"
+| "is_signed_integer_type (BabTy_MathInt _) = True"
+| "is_signed_integer_type _ = False"
+
+(* Check if a type is a finite integer type *)
+fun is_finite_integer_type :: "BabType \<Rightarrow> bool" where
+  "is_finite_integer_type (BabTy_FiniteInt _ _ _) = True"
+| "is_finite_integer_type _ = False"
+
+(* Finite integer types are ground *)
+lemma finite_integer_type_is_ground:
+  "is_finite_integer_type ty \<Longrightarrow> is_ground ty"
+  by (cases ty) auto
+
+(* Check if an array dimension is resolved (not BabDim_Fixed) *)
+fun is_resolved_dimension :: "BabDimension \<Rightarrow> bool" where
+  "is_resolved_dimension (BabDim_Fixed _) = False"
+| "is_resolved_dimension _ = True"
+
+(* Check if a type is a runtime-compatible type (no MathInt/MathReal) *)
+(* Note: Metavariables are considered runtime types, but metavariables should theoretically
+   be removed anyway, post type inference. *)
+fun is_runtime_type :: "BabType \<Rightarrow> bool" where
+  "is_runtime_type (BabTy_MathInt _) = False"
+| "is_runtime_type (BabTy_MathReal _) = False"
+| "is_runtime_type (BabTy_Name _ _ tyArgs) = list_all is_runtime_type tyArgs"
+| "is_runtime_type (BabTy_Tuple _ tys) = list_all is_runtime_type tys"
+| "is_runtime_type (BabTy_Record _ flds) = list_all (is_runtime_type \<circ> snd) flds"
+| "is_runtime_type (BabTy_Array _ ty _) = is_runtime_type ty"
+| "is_runtime_type _ = True"
+
+(* Signed integer types are integer types *)
+lemma signed_integer_type_is_integer_type:
+  "is_signed_integer_type ty \<Longrightarrow> is_integer_type ty"
+  by (cases ty) auto
+
+(* Finite integer types are integer types *)
+lemma finite_integer_type_is_integer_type:
+  "is_finite_integer_type ty \<Longrightarrow> is_integer_type ty"
+  by (cases ty) auto
+
+(* Integer types are either FiniteInt or MathInt *)
+lemma is_integer_type_cases:
+  assumes "is_integer_type ty"
+  obtains (FiniteInt) loc sign bits where "ty = BabTy_FiniteInt loc sign bits"
+        | (MathInt) loc where "ty = BabTy_MathInt loc"
+  using assms by (cases ty) auto
+
+(* Substituting runtime types preserves runtime-ness *)
+lemma is_runtime_type_substitute_bab_type:
+  assumes "is_runtime_type ty"
+      and "\<forall>ty' \<in> fmran' subst. is_runtime_type ty'"
+  shows "is_runtime_type (substitute_bab_type subst ty)"
+using assms proof (induction ty rule: is_runtime_type.induct)
+  (* BabTy_Name case - need to handle both variable substitution and recursive args *)
+  case (3 loc name tyArgs)
+  show ?case
+  proof (cases tyArgs)
+    case Nil
+    (* tyArgs = [], so this might be a type variable that gets substituted *)
+    then show ?thesis
+    proof (cases "fmlookup subst name")
+      case None
+      with Nil show ?thesis by simp
+    next
+      case (Some substTy)
+      with "3.prems"(2) have "is_runtime_type substTy"
+        by (simp add: fmran'I)
+      with Some Nil show ?thesis by simp
+    qed
+  next
+    case (Cons a list)
+    (* tyArgs is non-empty, so not substituted (just recurse on args) *)
+    from "3.prems"(1) Cons have args_rt: "list_all is_runtime_type (a # list)"
+      by simp
+    have "\<forall>t \<in> set (a # list). is_runtime_type (substitute_bab_type subst t)"
+    proof
+      fix t assume "t \<in> set (a # list)"
+      with args_rt have "is_runtime_type t"
+        using split_list by fastforce
+      with "3.IH" "3.prems"(2) Cons \<open>t \<in> set (a # list)\<close> show "is_runtime_type (substitute_bab_type subst t)"
+        by auto
+    qed
+    hence "list_all is_runtime_type (map (substitute_bab_type subst) (a # list))"
+      by (simp add: list_all_iff)
+    with Cons show ?thesis by simp
+  qed
+next
+  (* Tuple case *)
+  case (4 loc tys)
+  from "4.prems"(1) have "list_all is_runtime_type tys" by simp
+  hence "list_all is_runtime_type (map (substitute_bab_type subst) tys)"
+    using "4.IH" "4.prems"(2) by (auto simp: list_all_iff)
+  then show ?case by simp
+next
+  (* Record case *)
+  case (5 loc flds)
+  from "5.prems"(1) have "list_all (is_runtime_type \<circ> snd) flds" by simp
+  hence "list_all (is_runtime_type \<circ> snd) (map (\<lambda>(name, ty). (name, substitute_bab_type subst ty)) flds)"
+    using "5.IH" "5.prems"(2) by (auto simp: list_all_iff)
+  then show ?case by simp
+next
+  (* Array case *)
+  case (6 loc ty dims)
+  from "6.prems"(1) have "is_runtime_type ty" by simp
+  with "6.IH" "6.prems"(2) have "is_runtime_type (substitute_bab_type subst ty)" by simp
+  then show ?case by simp
+qed simp_all
+
+end
